examples/ProcFDInv.v
@@ -29,17 +29,97 @@ Section Invariants.
             (predictNextPc: forall ty, fullType ty (SyntaxKind (Bit addrSize)) -> (* pc *)
                                        Expr ty (SyntaxKind (Bit addrSize))).
 
-  (* Definition fetchDecodeInl := projT1 (fetchDecodeInl *)
-  (*                                        getOptype getLdDst getLdAddr getLdSrc calcLdAddr *)
-  (*                                        getStAddr getStSrc calcStAddr getStVSrc *)
-  (*                                        getSrc1 predictNextPc). *)
+  Definition fetchDecodeInl := projT1 (fetchDecodeInl
+                                         getOptype getLdDst getLdAddr getLdSrc calcLdAddr
+                                         getStAddr getStSrc calcStAddr getStVSrc
+                                         getSrc1 predictNextPc).
 
-  (* Record fetchDecode_inv (o: RegsT) : Prop := *)
-  (*   { pcv0 : fullType type (SyntaxKind (Bit addrSize)); *)
-  (*     Hpcv0 : M.find "pc"%string o = Some (existT _ _ pcv0); *)
-  (*     pgmv1 : fullType type (SyntaxKind (Vector (Data lgDataBytes) addrSize)); *)
-  (*     Hpgmv1 : M.find "pgm"%string o = Some (existT _ _ pgmv1); *)
-  (*     fepochv0 : fullType type (SyntaxKind Bool); *)
-  (*     Hfepochv0 : M.find "fEpoch"%string o = Some (existT _ _ fepochv0) }. *)
+  Definition fetchDecode_inv_body
+             (pcv: fullType type (SyntaxKind (Bit addrSize)))
+             (pgmv: fullType type (SyntaxKind (Vector (Data lgDataBytes) addrSize)))
+             (fepochv: fullType type (SyntaxKind Bool))
+             (f2dfullv: fullType type (SyntaxKind Bool))
+             (f2deltv: fullType type (SyntaxKind (f2dElt addrSize lgDataBytes))) :=
+    f2dfullv = true ->
+    let rawInst := f2deltv ``"rawInst" in
+    (rawInst = pgmv (f2deltv ``"curPc") /\
+     f2deltv ``"nextPc" = evalExpr (predictNextPc type (f2deltv ``"curPc")) /\
+     f2deltv ``"nextPc" = pcv /\
+     f2deltv ``"epoch" = fepochv).
+                                                      
+  Record fetchDecode_inv (o: RegsT) : Prop :=
+    { pcv : fullType type (SyntaxKind (Bit addrSize));
+      Hpcv : M.find "pc"%string o = Some (existT _ _ pcv);
+      pgmv : fullType type (SyntaxKind (Vector (Data lgDataBytes) addrSize));
+      Hpgmv : M.find "pgm"%string o = Some (existT _ _ pgmv);
+      fepochv : fullType type (SyntaxKind Bool);
+      Hfepochv : M.find "fEpoch"%string o = Some (existT _ _ fepochv);
+
+      f2dfullv : fullType type (SyntaxKind Bool);
+      Hf2dfullv : M.find "full.f2d"%string o = Some (existT _ _ f2dfullv);
+      f2deltv : fullType type (SyntaxKind (f2dElt addrSize lgDataBytes));
+      Hf2deltv : M.find "elt.f2d"%string o = Some (existT _ _ f2deltv);
+
+      Hinv : fetchDecode_inv_body pcv pgmv fepochv f2dfullv f2deltv
+    }.
+
+  Hint Unfold fetchDecode_inv_body : InvDefs.
+
+  Ltac fetchDecode_inv_old :=
+    repeat match goal with
+           | [H: fetchDecode_inv _ |- _] => destruct H
+           end;
+    kinv_red.
+
+  Ltac fetchDecode_inv_new :=
+    econstructor; (* let's prove that the invariant holds for the next state *)
+    try (findReify; (reflexivity || eassumption); fail);
+    kregmap_clear; (* for improving performance *)
+    kinv_red; (* unfolding invariant definitions *)
+    repeat (* cheaper than "intuition" *)
+      (match goal with
+       | [ |- _ /\ _ ] => split
+       end);
+    try eassumption; intros; try reflexivity;
+    intuition kinv_simpl; intuition idtac.
+
+  Ltac fetchDecode_inv_tac := fetchDecode_inv_old; fetchDecode_inv_new.
+
+  Lemma fetchDecode_inv_ok':
+    forall init n ll,
+      init = initRegs (getRegInits fetchDecodeInl) ->
+      Multistep fetchDecodeInl init n ll ->
+      fetchDecode_inv n.
+  Proof. (* SKIP_PROOF_ON
+    induction 2.
+
+    - fetchDecode_inv_old.
+      unfold getRegInits, fetchDecodeInl, ProcFDInl.fetchDecodeInl, projT1.
+      fetchDecode_inv_new; simpl in *; kinv_simpl.
+
+    - kinvert.
+      + mred.
+      + mred.
+      + kinv_dest_custom fetchDecode_inv_tac.
+      + kinv_dest_custom fetchDecode_inv_tac.
+      + kinv_dest_custom fetchDecode_inv_tac.
+      + kinv_dest_custom fetchDecode_inv_tac.
+      + kinv_dest_custom fetchDecode_inv_tac.
+      + kinv_dest_custom fetchDecode_inv_tac.
+
+        END_SKIP_PROOF_ON *) admit.
+  Qed.
+
+  Lemma fetchDecode_inv_ok:
+    forall o,
+      reachable o fetchDecodeInl ->
+      fetchDecode_inv o.
+  Proof.
+    intros; inv H; inv H0.
+    eapply fetchDecode_inv_ok'; eauto.
+  Qed.
 
 End Invariants.
+
+Hint Unfold fetchDecode_inv_body : InvDefs.
+
